WIP

proofs/itrees/it_exec.v
@@ -1,97 +1,4 @@
-(*
-From Coq Require Import
-     Arith.PeanoNat
-     Lists.List
-     Strings.String
-     Morphisms
-     Setoid
-     RelationClasses
-     EquivDec
-     Equality
-     Program.Tactics.
 
-From ExtLib Require Import
-     Data.String
-     Structures.Monad
-     Structures.Traversable
-     Data.List
-     Core.RelDec
-     Structures.Maps
-     Data.Map.FMapAList.
-
-From ITree Require Import
-     ITree
-     ITreeFacts
-     Monad
-     Basics.HeterogeneousRelations     
-     Events.Map
-     Events.State
-     Events.StateFacts
-     Events.Reader
-     Events.Exception
-     Events.FailFacts.
-
-Require Import Paco.paco.
-Require Import Psatz.
-Require Import ProofIrrelevance.
-Require Import FunctionalExtensionality.
-
-From mathcomp Require Import ssreflect ssrfun ssrbool ssrnat seq eqtype fintype.
-
-From ITree Require Import
-(*     Basics.Tacs *)
-     Basics.Category
-     Basics.Basics
-     Basics.Function
-     Core.ITreeDefinition
-     Core.KTree
-     Eq.Eqit
-     Eq.UpToTaus
-     Eq.Paco2
-     Indexed.Sum
-     Indexed.Function
-     Indexed.Relation
-     Interp.Handler
-     Interp.Interp
-     Interp.InterpFacts
-     Interp.Recursion.
-
-From ITree Require Import Rutt RuttFacts.
-
-From ITree Require Import EqAxiom.
-
-From Jasmin Require Import utils. (* expr psem_defs psem oseq. *)
-
-Import Monads.
-Import MonadNotation.
-Local Open Scope monad_scope.
-Local Open Scope option_scope.
-
-Obligation Tactic := done || idtac.
-
-*)
-
-
-(* This files contains the monad transformer associated with exec *)
-
-(*
-(***)
-(* local redefinition of utils.result, to try circumvent the universe
-problem *)
-Variant result (E: Type) (A : Type) : Type :=
-    Ok of A | Error of E.
-
-Arguments Error {E} {A} s.
-Arguments Ok E [A] s.
-
-Definition exec t := result error t.
-(***)
-*)
-(*
-About MonadLawsE.
-About mathcomp.ssreflect.seq.
-About result.
-*)
 
 (* begin hide *)
 From Coq Require Import
@@ -125,9 +32,19 @@ Import ITreeNotations.
 Import ITree.Basics.Basics.Monads.
 Local Open Scope itree_scope.
 
-Set Universe Polymorphism.
+Set Implicit Arguments.
+Unset Strict Implicit.
+Unset Printing Implicit Defensive.
+
+(* Set Universe Polymorphism. *)
 
 Import Monads.
+
+Definition error_data := (error * unit)%type.
+
+Variant execS (A:Type) :=
+  | ESok : A -> execS A
+  | ESerror : error_data -> execS A.
 
 Section ExecT.
 
@@ -135,69 +52,65 @@ Section ExecT.
     {MIm : MonadIter m}.
 
   Definition execT (m : Type -> Type) (a : Type) : Type :=
-    m (exec a)%type.
+    m (execS a)%type.
 
   Global Instance execT_fun : Functor.Functor (execT m) :=
     {| Functor.fmap :=
-        fun X Y (f: X -> Y) => 
+        fun X Y (f: X -> Y) =>
           Functor.fmap (fun x =>
                           match x with
-                          | Error e => Error e
-                          | Ok x => @Ok error Y (f x) end) |}.
+                          | ESerror e => ESerror _ e
+                          | ESok x => ESok (f x) end) |}.
 
   Global Instance execT_monad : Monad (execT m) :=
-    {| ret := fun _ x => @ret m _ _ (Ok _ x);
+    {| ret := fun _ x => @ret m _ _ (ESok x);
        bind := fun _ _ c k =>
-                 bind (m := m) c 
+                 bind (m := m) c
                    (fun x => match x with
-                             | Error e => @ret m _ _ (Error e)
-                             | Ok x => k x end)
+                             | ESerror e => @ret m _ _ (ESerror _ e)
+                             | ESok x => k x end)
     |}.
 
   Global Instance execT_iter  : MonadIter (execT m) :=
-    fun A I body i => Basics.iter (M := m) (I := I) (R := exec A) 
+    fun A I body i => Basics.iter (M := m) (I := I) (R := execS A)
       (fun i => bind (m := m)
                (body i)
                (fun x => match x with
-                         | Error e       => ret (inr (Error e))
-                         | Ok (inl j) => @ret m _ _ (inl j)
-                         | Ok (inr a) => @ret m _ _ (inr (Ok _ a))
+                         | ESerror e       => ret (inr (ESerror _ e))
+                         | ESok (inl j) => @ret m _ _ (inl j)
+                         | ESok (inr a) => @ret m _ _ (inr (ESok a))
                          end)) i.
 
 End ExecT.
 
+Section ExecTLaws.
 
-Section ExecTLaws. 
 
-
-Definition result_rel (W: Set) {X} (R : relation X) (Re : relation W) :
-   relation (result W X) :=
-fun (mx my : result W X) =>
+Definition execS_rel {X} (R : relation X) (Re : relation error_data) :
+   relation (execS X) :=
+fun (mx my : execS X) =>
 match mx with
-| Ok x => match my with
-            | Ok y => R x y
-            | Error _ => False
+| ESok x => match my with
+            | ESok y => R x y
+            | ESerror _ => False
             end
-| Error e0 => match my with
-          | Ok _ => False
-          | Error e1 => Re e0 e1 
+| ESerror e0 => match my with
+          | ESok _ => False
+          | ESerror e1 => Re e0 e1
           end
 end.
 
-Lemma result_rel_eq (W: Set) : forall {A : Type},
-    eq_rel (@eq (result W A)) (result_rel W eq eq).
+Lemma execS_rel_eq : forall {A : Type},
+    eq_rel (@eq (execS A)) (execS_rel eq eq).
 Proof.
   intros ?; split; intros [] [] EQ; subst; try inv EQ; cbn; auto.
 Qed.
 
-Definition exec_rel' {X: Type} (R : relation X) :
-   relation (exec X) := result_rel error R (fun x y => True). 
-
 Definition exec_rel {X: Type} (R : relation X) :
-   relation (exec X) := result_rel error R eq. 
+   relation (execS X) := execS_rel R eq.
 
 Lemma exec_rel_eq : forall {A : Type},
-    eq_rel (@eq (exec A)) (exec_rel eq).
+    eq_rel (@eq (execS A)) (exec_rel eq).
 Proof.
   intros ?; split; intros [] [] EQ; subst; try inv EQ; cbn; auto.
 Qed.
@@ -241,17 +154,17 @@ Global Instance MonadLaws_execE {E} : MonadLawsE (execT (itree E)).
       rewrite <- (bind_ret_r x) at 2.
       eapply eutt_eq_bind; intros []; reflexivity.
     - intros; cbn; rewrite bind_bind.
-      eapply eutt_eq_bind; intros []. 
-      + eapply eutt_eq_bind; intros []; reflexivity. 
+      eapply eutt_eq_bind; intros [].
+      + eapply eutt_eq_bind; intros []; reflexivity.
       + rewrite bind_ret_l; reflexivity.
     - repeat intro; cbn.
       eapply eutt_clo_bind; eauto.
       intros [] [] REL; cbn in *; subst; try contradiction.
       + apply H0.
-      + setoid_rewrite <- eutt_Ret. 
+      + setoid_rewrite <- eutt_Ret.
         reflexivity.
   Qed.
-  
+
 End ExecTLaws.
 
 Definition interp_exec {E M}
@@ -280,7 +193,7 @@ Proof.
   cbn; repeat (rewrite ?bind_bind, ?bind_ret_l, ?bind_map; try reflexivity).
   cbn; repeat (rewrite ?bind_bind, ?bind_ret_l, ?bind_map; try reflexivity).
   cbn; repeat (rewrite ?bind_bind, ?bind_ret_l, ?bind_map; try reflexivity).
-  apply eq_itree_clo_bind with (UU := Logic.eq); [reflexivity | intros x ? <-]. 
+  apply eq_itree_clo_bind with (UU := Logic.eq); [reflexivity | intros x ? <-].
   destruct x as [x|].
   - rewrite bind_ret_l; reflexivity.
   - rewrite bind_ret_l; reflexivity.
@@ -290,7 +203,7 @@ Global Instance interp_exec_eq_itree {X E F} {R : X -> X -> Prop}
   (h : E ~> execT (itree F)) :
   Proper (eq_itree R ==> eq_itree (exec_rel R)) (@interp_exec _ _ _ _ _ h X).
 Proof.
-  repeat red. 
+  repeat red.
   ginit.
   pcofix CIH.
   intros s t EQ.
@@ -299,7 +212,7 @@ Proof.
   destruct EQ; cbn; subst; try discriminate; pclearbot; try (gstep; constructor; eauto with paco; fail).
   guclo eqit_clo_bind; econstructor; [reflexivity | intros x ? <-].
   destruct x as [x|]; gstep; econstructor; eauto with paco itree.
-  unfold exec_rel, result_rel; auto.
+  unfold exec_rel, execS_rel; auto.
 Qed.
 
 (* Convenient special case: [option_rel eq eq] is equivalent to [eq], so we can avoid bothering *)
@@ -307,14 +220,14 @@ Global Instance interp_exec_eq_itree_eq {X E F} (h : E ~> execT (itree F)) :
   Proper (eq_itree eq ==> eq_itree eq) (@interp_exec _ _ _ _ _ h X).
 Proof.
   repeat intro.
-  setoid_rewrite result_rel_eq.
+  setoid_rewrite execS_rel_eq.
   apply interp_exec_eq_itree; auto.
 Qed.
 
 Global Instance interp_exec_eutt {X E F R} (h : E ~> execT (itree F)) :
   Proper (eutt R ==> eutt (exec_rel R)) (@interp_exec _ _ _ _ _ h X).
 Proof.
-  repeat red. 
+  repeat red.
   einit.
   ecofix CIH.
   intros s t EQ.
@@ -325,7 +238,7 @@ Proof.
     intros [] [] EQ; inv EQ.
     + estep; ebase.
     + eret.
-    + reflexivity.  
+    + reflexivity.
   - rewrite tau_euttge, unfold_interp_exec; eauto.
   - rewrite tau_euttge, unfold_interp_exec; eauto.
 Qed.
@@ -344,12 +257,12 @@ Lemma interp_exec_tau {E F R} {f : E ~> execT (itree F)} (t: itree E R):
 Proof. rewrite unfold_interp_exec. reflexivity. Qed.
 
 Lemma interp_exec_vis {E F : Type -> Type} {T U : Type}
-      (e : E T) (k : T -> itree E U) (h : E ~> execT (itree F)) 
-  : interp_exec h (Vis e k) 
+      (e : E T) (k : T -> itree E U) (h : E ~> execT (itree F))
+  : interp_exec h (Vis e k)
                 ≅ h T e >>= fun mx =>
                               match mx with
-                              | Error e => Ret (Error e)
-                              | Ok x => Tau (interp_exec h (k x))
+                              | ESerror e => Ret (ESerror _ e)
+                              | ESok x => Tau (interp_exec h (k x))
                               end.
 Proof.
   rewrite unfold_interp_exec. reflexivity.
@@ -363,7 +276,7 @@ Qed.
      With the latter, we need to be more rigorous with the infrastructure.
  *)
 Lemma interp_exec_Ret : forall {X E F} (h : E ~> execT (itree F)) (x : X),
-    interp_exec h (Ret x) ≅ Ret (Ok _ x).
+    interp_exec h (Ret x) ≅ Ret (ESok x).
 Proof.
   intros; rewrite unfold_interp_exec; reflexivity.
 Qed.
@@ -375,7 +288,7 @@ Proof.
 Qed.
 
 Lemma interp_exec_trigger {E F : Type -> Type} {R : Type}
-      (e : E R) (f : E ~> execT (itree F)) 
+      (e : E R) (f : E ~> execT (itree F))
   : interp_exec f (ITree.trigger e) ≈ f _ e.
 Proof.
   unfold ITree.trigger. rewrite interp_exec_vis.
@@ -391,7 +304,7 @@ Qed.
 Lemma interp_exec_bind : forall {X Y E F} (t : itree _ X) (k : X -> itree _ Y) (h : E ~> execT (itree F)),
     interp_exec h (ITree.bind t k) ≅
                 ITree.bind (interp_exec h t)
-                (fun mx => match mx with | (Error e) => ret (Error e) | Ok x => interp_exec h (k x) end).
+                (fun mx => match mx with | (ESerror e) => ret (ESerror _ e) | ESok x => interp_exec h (k x) end).
 Proof.
   intros X Y E F; ginit; pcofix CIH; intros.
   rewrite unfold_bind.
