proofs/itrees/it_sems_core.v
@@ -4,6 +4,7 @@ From Jasmin Require Import oseq.
 From Jasmin Require Import expr.
 From Jasmin Require Import it_jasmin_lib.
 
+(* FIXME clean this *)
 From Coq Require Import
      Arith.PeanoNat
      Lists.List
@@ -28,7 +29,7 @@ From ITree Require Import
      ITree
      ITreeFacts
      Monad
-     Basics.HeterogeneousRelations     
+     Basics.HeterogeneousRelations
      Events.Map
      Events.State
      Events.StateFacts
@@ -65,11 +66,11 @@ From ITree Require Import Rutt RuttFacts.
 From ITree Require Import EqAxiom.
 
 From Jasmin Require Import expr psem_defs psem oseq.
-From Jasmin Require Import it_gen_lib it_jasmin_lib.
+From Jasmin Require Import it_gen_lib it_jasmin_lib it_exec.
 From Jasmin Require Import compiler_util.
 (* problematic *)
-From Jasmin Require Import it_exec_mono.
 
+(* End FIXME *)
 Import Monads.
 Import MonadNotation.
 Local Open Scope monad_scope.
@@ -81,8 +82,6 @@ Unset Printing Implicit Defensive.
 
 (* Set Universe Polymorphism. *)
 
-Obligation Tactic := done || idtac.
-
 (* This files contains semantic models distinguished by use of either
 mutual or double recursion, and by either modular, error-aware or flat
 structure. There are fives models (MM: mutual modular; ME: mutual
@@ -90,72 +89,79 @@ error; MF: mutual flat; DE: double error; DF double flat) *)
 
 (**** ERROR SEMANTICS *******************************************)
 Section Errors.
-  
+
 (* type of errors (this might becom richer) *)
   (* Variant ErrType : Type := Err : ErrType. *)
-Notation ErrType1 := (error).
-Notation ErrType2 := (option pp_error_loc).
-Notation Err := (ErrType).
-
 (* error events *)
-Definition ErrState : Type -> Type := exceptE ErrType1.
-Definition CErrState : Type -> Type := exceptE ErrType2.
+
+
+Definition ErrEvent : Type -> Type := exceptE error_data.
+
+(*
+sem_I : prog -> estate -> instr -> itree syscall_Event (state_error + estate)
+sem_i : prog -> estate -> instr_r -> itree syscall_Event (state_error + estate)
+sem_c : prog -> estate -> cmd -> itree syscall_Event (state_error + estate)
+sem_fun : prog -> mem -> syscall -> funname -> values -> itree syscall_Event (state_error + (mem * syscall * values))
+*)
 
 (* failT (itree E) R = itree E (option R) *)
-Definition handle_Err {E} : ErrState ~> failT (itree E) :=
-  fun _ _ => Ret (None).
+Definition handle_Err {E} : ErrEvent ~> execT (itree E) :=
+  fun _ e =>
+    match e with
+    | Throw e' => Ret (ESerror _ e')
+    end.
 
 (* Err handler *)
 Definition ext_handle_Err {E: Type -> Type} :
-  ErrState +' E ~> failT (itree E) :=
+  ErrEvent +' E ~> execT (itree E) :=
   fun _ e =>
   match e with
   | inl1 e' => handle_Err e'
-  | inr1 e' => Vis e' (pure (fun x => Some x)) end.                        
+  | inr1 e' => Vis e' (pure (fun x => ESok x)) end.
 
-(* ErrState interpreter *)
-Definition interp_Err {E: Type -> Type} {A}  
-  (t: itree (ErrState +' E) A) : failT (itree E) A :=
-  interp_fail ext_handle_Err t.
-
+(* ErrEvent interpreter *)
+Definition interp_Err {E: Type -> Type} {A}
+  (t: itree (ErrEvent +' E) A) : execT (itree E) A :=
+  interp_exec ext_handle_Err t.
 
 (*** auxiliary error functions *)
-
-Definition err_get {E: Type -> Type} `{ErrState -< E} {S} {V}
+(* FIXME: change this name *)
+Definition err_get {E: Type -> Type} `{ErrEvent -< E} {S} {V} (Err: S -> error_data )
   (f: S -> option V) : stateT S (itree E) V :=
   fun st => match (f st) with
             | Some v => Ret (st, v)
-            | None => throw Err end.                
-
-Definition err_put {E: Type -> Type} `{ErrState -< E} {S}
+            | None => throw (Err st) end.
+(*
+Definition err_put {E: Type -> Type} `{ErrEvent -< E} {S}
   (f: S -> option S) : stateT S (itree E) unit :=
   fun st => match (f st) with
             | Some st' => Ret (st', tt)
-            | None => throw Err end.                
+            | None => throw Err end.
 
-Definition err_write {E: Type -> Type} `{ErrState -< E} {S}
+Definition err_write {E: Type -> Type} `{ErrEvent -< E} {S}
   (ms: option S) : stateT S (itree E) unit :=
   fun st => match ms with
             | Some st' => Ret (st', tt)
-            | None => throw Err end.                
-
-Definition err_opt {E: Type -> Type} `{ErrState -< E} :
+            | None => throw Err end.
+*)
+(*
+Definition err_opt {E: Type -> Type} `{ErrEvent -< E} :
   option ~> itree E :=
   fun _ t => match t with
              | Some v => Ret v
-             | None => throw Err end.                
+             | None => throw Err end.
 
-Definition err_st_opt {E: Type -> Type} `{ErrState -< E} {S} :
+Definition err_st_opt {E: Type -> Type} `{ErrEvent -< E} {S} :
   option ~> stateT S (itree E) :=
   fun _ t st => match t with
                 | Some v => Ret (st, v)
-                | None => throw Err end.                
-
-Definition err_result {E: Type -> Type} `{ErrState -< E} T :
-  result T ~> itree E :=
+                | None => throw Err end.
+*)
+Definition err_result {E: Type -> Type} `{ErrEvent -< E} (Err : error -> error_data) :
+  result error ~> itree E :=
   fun _ t => match t with
              | Ok v => Ret v
-             | Error _ => throw Err end.                
+             | Error e => throw (Err e) end.
 
 End Errors.
 
@@ -166,16 +172,12 @@ End Errors.
 Section Lang.
 Context (asm_op: Type) (asmop: asmOp asm_op).
 
-(* reader events *)
-Variant FunE : Type -> Type :=
-  | FunCode (fn : funname) : FunE cmd.                               
-
 
 (**********************************************************************)
 (********** EVENT SEMANTICS ******************************************)
 
 Section WSW.
-Context {wsw: WithSubWord}.   
+Context {wsw: WithSubWord}.
 Context
   (dc: DirectCall)
   (syscall_state : Type)
@@ -186,191 +188,215 @@ Context
   (scP : semCallParams)
   (ev : extra_val_t).
 
-Section OneProg.  
+Section OneProg.
 Context (pr : prog).
 
 
 (***** FUN-READER SEMANTICS ******************************************)
 (* Section ModularSem. *)
 
-Definition FunDef : Type := _fundef extra_fun_t.
-
-Definition get_FunDef (fn: funname) : option FunDef :=
-  get_fundef (p_funcs pr) fn.
-
-Definition funCode (f: FunDef) : cmd := 
-  @f_body asm_op asmop extra_fun_t f.
-
-Definition get_FunCode (fn: funname) : option cmd := 
+(*
+Definition get_FunCode (fn: funname) : option cmd :=
   opt_lift (@f_body asm_op asmop extra_fun_t) (get_FunDef fn).
 
 Definition get_FunDests (fn: funname) : option lvals :=
-  get_FunDef fn >>o= fun f => Some (map Lvar (f.(f_res))). 
-
-Definition handle_FunE {E: Type -> Type}
-  `{ErrState -< E} : FunE ~> itree E :=
-  fun _ e =>
-    match e with
-    | FunCode fn => err_opt (get_FunCode fn) end.   
-
-Definition ext_handle_FunE {E: Type -> Type} `{ErrState -< E} :
-  FunE +' E ~> itree E :=
-  case_ handle_FunE (id_ E).
-
-(* FunE interpreter *)
-Definition interp_FunE {E: Type -> Type} {X: ErrState -< E}
-  {A: Type}
-  (t : itree (FunE +' E) A) : itree E A :=
-  interp ext_handle_FunE t.
-
+  get_FunDef fn >>o= fun f => Some (map Lvar (f.(f_res))).
+*)
 
 (***** INSTR AUX FUNCTIONS *******************************************)
 
 (** Ccall *)
-
-Definition ret_get_FunDef {E: Type -> Type} 
+(*
+Definition ret_get_FunDef {E: Type -> Type}
   (fn: funname) : execT (itree E) FunDef :=
-  Ret (o2r ErrType (get_FunDef fn)).           
+  Ret (o2r ErrType (get_FunDef fn)).
+*)
 
-Definition err_get_FunDef {E} `{ErrState -< E}
-  (fn: funname) : itree E FunDef :=
-  err_opt (get_FunDef fn).           
+Definition mk_error_data (s:estate) (e:error)  := (e, tt).
+
+Definition mk_errtype := fun s => mk_error_data s ErrType.
+
+Definition iget_fundef {E} `{ErrEvent -< E}
+  (fn: funname) : stateT estate (itree E) fundef :=
+  err_get mk_errtype (fun _ => get_fundef (p_funcs pr) fn).
+
+Definition iresult  {E} `{ErrEvent -< E} {T} (F : estate -> exec T) (s:estate) : itree E T :=
+  err_result (mk_error_data s) (F s).
 
 
-Definition ret_get_FunCode {E: Type -> Type}
+Definition iwrite_var {E} `{ErrEvent -< E}
+   (wdb : bool) (x : var_i) (v : value) (s : estate) : itree E estate :=
+  iresult (write_var wdb x v) s.
+
+Definition iwrite_lval {E} `{ErrEvent -< E}
+   (wdb : bool) (gd : glob_decls) (x : lval) (v : value) (s : estate) : itree E estate :=
+  iresult (write_lval wdb gd x v) s.
+
+Definition iwrite_lvals {E} `{ErrEvent -< E}
+   (wdb : bool) (gd : glob_decls) (s : estate) (xs : lvals) (vs : values) : itree E estate :=
+  iresult (fun s => write_lvals wdb gd s xs vs) s.
+
+Definition isem_pexpr {E} `{ErrEvent -< E}
+   (wdb : bool) (gd : glob_decls) (s : estate) (e: pexpr) : itree E value :=
+  iresult (fun s => sem_pexpr wdb gd s e) s.
+
+Definition isem_pexprs {E} `{ErrEvent -< E}
+   (wdb : bool) (gd : glob_decls) (s : estate) (es: pexprs) : itree E values :=
+  iresult (fun s => sem_pexprs wdb gd s es) s.
+
+
+
+
+
+
+(*Definition ret_get_FunCode {E: Type -> Type}
   (fn: funname) : execT (itree E) cmd :=
   f <- ret_get_FunDef fn ;;
   Ret (ok (funCode f)).
 
-Definition err_get_FunCode {E} `{ErrState -< E}
+Definition err_get_FunCode {E} `{ErrEvent -< E}
   (fn: funname) : itree E cmd :=
   f <- err_get_FunDef fn ;;
   Ret (funCode f).
-
+*)
+(*
 Definition pure_eval_Args (args: pexprs) (st: estate) :
-  exec (seq value) := 
+  exec (seq value) :=
   sem_pexprs (~~direct_call) (p_globs pr) st args.
 
 Definition truncate_Args (f: FunDef) (vargs: seq value) :
   exec (seq value) :=
   mapM2 ErrType dc_truncate_val f.(f_tyin) vargs.
+*)
 
-Definition err_eval_Args {E} `{ErrState -< E}
+(*
+Definition err_eval_Args {E} `{ErrEvent -< E}
   (fn: funname) (args: pexprs) (st0: estate) : itree E (seq value) :=
   f <- err_get_FunDef fn ;;
   vargs' <- err_result (pure_eval_Args args st0) ;;
   err_result (truncate_Args f vargs').
-  
-Definition err_init_state {E} `{ErrState -< E}
-   (fn: funname) (vargs: seq value) (st0: estate) : itree E estate :=   
+
+Definition err_init_state {E} `{ErrEvent -< E}
+   (fn: funname) (vargs: seq value) (st0: estate) : itree E estate :=
   let scs1 := st0.(escs) in
   let m1 := st0.(emem) in
   f <- err_get_FunDef fn ;;
-  st1 <- err_result 
+  st1 <- err_result
        (init_state f.(f_extra) (p_extra pr) ev (Estate scs1 m1 Vm.init)) ;;
-  err_result 
+  err_result
       (write_vars (~~direct_call) (f_params f) vargs st1).
 
-Definition err_return_val {E} `{ErrState -< E}
+Definition err_return_val {E} `{ErrEvent -< E}
   (fn: funname) (st0: estate) : itree E (seq value) :=
   f <- err_get_FunDef fn ;;
-  vres <- err_result 
+  vres <- err_result
       (get_var_is (~~ direct_call) st0.(evm) f.(f_res)) ;;
-  err_result 
+  err_result
       (mapM2 ErrType dc_truncate_val f.(f_tyout) vres).
 
-Definition err_reinstate_caller {E} `{ErrState -< E}
+Definition err_reinstate_caller {E} `{ErrEvent -< E}
   (fn: funname) (xs: lvals) (vres: seq value)
   (st_ee st_er: estate) : itree E estate :=
   f <- err_get_FunDef fn ;;
   let scs2 := st_ee.(escs) in
-  let m2 := finalize f.(f_extra) st_ee.(emem) in      
-  err_result 
+  let m2 := finalize f.(f_extra) st_ee.(emem) in
+  err_result
          (write_lvals (~~direct_call) (p_globs pr)
                       (with_scs (with_mem st_er m2) scs2) xs vres).
-
-Definition ret_eval_Args {E: Type -> Type} 
+*)
+(*
+Definition ret_eval_Args {E: Type -> Type}
   (fn: funname) (args: pexprs) (st0: estate) : execT (itree E) (seq value) :=
-  f <- ret_get_FunDef fn ;; 
+  f <- ret_get_FunDef fn ;;
   Ret (Let vargs' := pure_eval_Args args st0 in truncate_Args f vargs').
 
-Definition ret_init_state {E: Type -> Type} 
-   (fn: funname) (vargs: seq value) (st0: estate) : execT (itree E) estate :=   
+Definition ret_init_state {E: Type -> Type}
+   (fn: funname) (vargs: seq value) (st0: estate) : execT (itree E) estate :=
   let scs1 := st0.(escs) in
   let m1 := st0.(emem) in
-  f <- ret_get_FunDef fn ;; 
-  Ret 
+  f <- ret_get_FunDef fn ;;
+  Ret
   (Let st1 := init_state f.(f_extra) (p_extra pr) ev (Estate scs1 m1 Vm.init) in
    write_vars (~~direct_call) (f_params f) vargs st1).
 
-Definition ret_return_val {E: Type -> Type} 
+Definition ret_return_val {E: Type -> Type}
   (fn: funname) (st0: estate) : execT (itree E) (seq value) :=
-  f <- ret_get_FunDef fn ;; 
-  Ret           
+  f <- ret_get_FunDef fn ;;
+  Ret
   (Let vres := get_var_is (~~ direct_call) st0.(evm) f.(f_res) in
    mapM2 ErrType dc_truncate_val f.(f_tyout) vres).
 
-Definition ret_reinstate_caller {E: Type -> Type} 
+Definition ret_reinstate_caller {E: Type -> Type}
   (fn: funname) (xs: lvals) (vres: seq value)
   (st_ee st_er: estate) : execT (itree E) estate :=
-  f <- ret_get_FunDef fn ;;   
+  f <- ret_get_FunDef fn ;;
   let scs2 := st_ee.(escs) in
-  let m2 := finalize f.(f_extra) st_ee.(emem) in      
+  let m2 := finalize f.(f_extra) st_ee.(emem) in
   Ret (write_lvals (~~direct_call) (p_globs pr)
                       (with_scs (with_mem st_er m2) scs2) xs vres).
-
+*)
 (** WriteIndex *)
-Definition ret_mk_WriteIndex {E} 
-  (x: var_i) (z: Z) (st1: estate) : execT (itree E) estate :=  
-    Ret (write_var true x (Vint z) st1).                             
-
-Definition err_mk_WriteIndex {E} `{ErrState -< E}
-  (x: var_i) (z: Z) (st1: estate) : itree E estate :=  
-    err_result (write_var true x (Vint z) st1).                             
+(*
+Definition ret_mk_WriteIndex {E}
+  (x: var_i) (z: Z) (st1: estate) : execT (itree E) estate :=
+    Ret (write_var true x (Vint z) st1).
+*)
+(*
+Definition err_mk_WriteIndex {E} `{ErrEvent -< E}
+  (x: var_i) (z: Z) (st1: estate) : itree E estate :=
+    err_result (write_var true x (Vint z) st1).
 
 (** EvalCond *)
-Definition ret_mk_EvalCond {E} 
+Definition ret_mk_EvalCond {E}
   (e: pexpr) (st1: estate) : execT (itree E) bool :=
-   let vv := sem_pexpr true (p_globs pr) st1 e in                               
+   let vv := sem_pexpr true (p_globs pr) st1 e in
    match vv with
    | Ok (Vbool bb) => ret (ok bb)
-   | _ => ret (Error ErrType) end.                       
+   | _ => ret (Error ErrType) end.
 
-Definition err_mk_EvalCond {E} `{ErrState -< E}
+Definition err_mk_EvalCond {E} `{ErrEvent -< E}
   (e: pexpr) (st1: estate) : itree E bool :=
-   let vv := sem_pexpr true (p_globs pr) st1 e in                               
+   let vv := sem_pexpr true (p_globs pr) st1 e in
    match vv with
    | Ok (Vbool bb) => ret bb
-   | _ => throw ErrType end.                       
+   | _ => throw ErrType end.
 
 
 (** EvalBound *)
-Definition ret_mk_EvalBound {E} 
+Definition ret_mk_EvalBound {E}
   (e: pexpr) (st1: estate) : execT (itree E) Z :=
-   let vv := sem_pexpr true (p_globs pr) st1 e in                               
+   let vv := sem_pexpr true (p_globs pr) st1 e in
    match vv with
    | Ok (Vint zz) => ret (ok zz)
-   | _ => ret (Error ErrType) end.                       
+   | _ => ret (Error ErrType) end.
 
-Definition err_mk_EvalBound {E} `{ErrState -< E}
+Definition err_mk_EvalBound {E} `{ErrEvent -< E}
   (e: pexpr) (st1: estate) : itree E Z :=
-   let vv := sem_pexpr true (p_globs pr) st1 e in                               
+   let vv := sem_pexpr true (p_globs pr) st1 e in
    match vv with
    | Ok (Vint zz) => ret zz
-   | _ => throw ErrType end.                       
+   | _ => throw ErrType end.
 
+*)
 
 (** AssgnE *)
 (* terminating *)
-Definition ret_mk_AssgnE {E: Type -> Type} 
-  (x: lval) (tg: assgn_tag) (ty: stype) (e: pexpr) 
-  (st1: estate) : execT (itree E) estate := Ret
-   (Let v := sem_pexpr true (p_globs pr) st1 e in 
+
+Definition eval_assgn
+  (x: lval) (tg: assgn_tag) (ty: stype) (e: pexpr)
+  (st1: estate) : exec estate :=
+   (Let v := sem_pexpr true (p_globs pr) st1 e in
     Let v' := truncate_val ty v in
     write_lval true (p_globs pr) x v' st1).
 
-Definition err_mk_AssgnE {E: Type -> Type} `{ErrState -< E}
-  (x: lval) (tg: assgn_tag) (ty: stype) (e: pexpr) 
+Definition ieval_assgn {E} `{ErrEvent -< E}
+ (x: lval) (tg: assgn_tag) (ty: stype) (e: pexpr)
+  (s: estate) : itree E estate :=
+  iresult (eval_assgn x tg ty e) s.
+
+(*
+Definition err_mk_AssgnE {E: Type -> Type} `{ErrEvent -< E}
+  (x: lval) (tg: assgn_tag) (ty: stype) (e: pexpr)
   (st1: estate) : itree E estate :=
     v <- err_result (sem_pexpr true (p_globs pr) st1 e) ;;
     v' <- err_result (truncate_val ty v) ;;
@@ -379,12 +405,12 @@ Definition err_mk_AssgnE {E: Type -> Type} `{ErrState -< E}
 
 (** OpnE *)
 (* terminating *)
-Definition ret_mk_OpnE {E: Type -> Type} 
+Definition ret_mk_OpnE {E: Type -> Type}
   (xs: lvals) (tg: assgn_tag) (o: sopn)
   (es : pexprs) (st1: estate) : execT (itree E) estate := Ret
     (sem_sopn (p_globs pr) o st1 xs es).
 
-Definition err_mk_OpnE {E: Type -> Type} `{ErrState -< E}
+Definition err_mk_OpnE {E: Type -> Type} `{ErrEvent -< E}
   (xs: lvals) (tg: assgn_tag) (o: sopn)
    (es : pexprs) (st1: estate) : itree E estate :=
     err_result (sem_sopn (p_globs pr) o st1 xs es).
@@ -392,17 +418,24 @@ Definition err_mk_OpnE {E: Type -> Type} `{ErrState -< E}
 
 (** SyscallE *)
 (* terminating *)
-Definition ret_mk_SyscallE {E: Type -> Type}
-  (xs: lvals) (o: syscall_t)
-  (es: pexprs) (st1: estate) : execT (itree E) estate := Ret 
-   (Let ves := sem_pexprs true (p_globs pr) st1 es in 
-    Let r3 := exec_syscall st1.(escs) st1.(emem) o ves in 
-    match r3 with
-    | (scs, m, vs) =>
-        write_lvals true (p_globs pr)
-                    (with_scs (with_mem st1 m) scs) xs vs end).
+*)
 
-Definition err_mk_SyscallE {E: Type -> Type} `{ErrState -< E}
+Definition eval_syscall
+   (xs: lvals) (o: syscall_t)
+   (es: pexprs) (s: estate) : exec estate :=
+  Let ves := sem_pexprs true (p_globs pr) s es in
+  Let: (scs, m, vs) := exec_syscall s.(escs) s.(emem) o ves in
+  write_lvals true (p_globs pr)
+     (with_scs (with_mem s m) scs) xs vs.
+
+(*
+Definition ieval_syscall {E} `{ErrEvent -< E}
+   (xs: lvals) (o: syscall_t)
+   (es: pexprs) (s: estate) : exec estate
+  iresult (eval_syscall
+*)
+(*
+Definition err_mk_SyscallE {E: Type -> Type} `{ErrEvent -< E}
   (xs: lvals) (o: syscall_t) (es: pexprs) (st1: estate) :
   itree E estate :=
     ves <- err_result (sem_pexprs true (p_globs pr) st1 es ) ;;
@@ -411,7 +444,7 @@ Definition err_mk_SyscallE {E: Type -> Type} `{ErrState -< E}
     | (scs, m, vs) =>
         err_result (write_lvals true (p_globs pr)
                        (with_scs (with_mem st1 m) scs) xs vs) end.
-
+*)
 
 (*** INTERPRETERS WITH ERROR (quasi-flat) ******************************)
 Section ErrorAwareSem.
@@ -419,23 +452,24 @@ Section ErrorAwareSem.
 (** Auxiliary functions for recursion on list (seq) *)
 
 Fixpoint st_cmd_map_r {E} (R: instr_r -> estate -> itree E estate)
-  (c: cmd) (st: estate) : itree E estate := 
-  match c with 
-  | nil => Ret st 
+  (c: cmd) (st: estate) : itree E estate :=
+  match c with
+  | nil => Ret st
   | (MkI _ i) :: c' => st' <- R i st ;; st_cmd_map_r R c' st'
   end.
 
-Fixpoint eval_for {E} `{ErrState -< E}
-  (R: cmd -> estate -> itree E estate)                
+Fixpoint eval_for {E} `{ErrEvent -< E}
+  (eval_cmd_ : cmd -> estate -> itree E estate)
   (i: var_i) (c: cmd)
-  (ls: list Z) (st: estate) : itree E estate :=
+  (ls: list Z) : estate -> itree E estate :=
     match ls with
-    | nil => fun st' => ret st'
-    | (w :: ws) => fun st' =>
-                     st1 <- err_mk_WriteIndex i w st' ;;
-                     st2 <- R c st1 ;;
-                     eval_for R i c ws st2
-    end st.
+    | nil => fun s => ret s
+    | (w :: ws) =>
+      fun s =>
+        s <- iwrite_var true i (Vint w) s;;
+        s <- eval_cmd_ c s;;
+        eval_for eval_cmd_ i c ws s
+    end.
 
 
 (**********************************************************************)
@@ -443,42 +477,81 @@ Fixpoint eval_for {E} `{ErrState -< E}
 Section With_MREC_error.
 
 (* mutual recursion events *)
+(* FIXME : should we find a better name ? *)
 Variant FCState : Type -> Type :=
  | FLCode (c: cmd) (st: estate) : FCState estate
- | FFCall (xs: lvals) (f: funname) (es: pexprs) (st: estate) : FCState estate.
-  
+ | FFCall (scs : syscall_state_t) (m:mem)
+          (f: funname) (vs:values) : FCState (syscall_state_t * mem * values).
+
 Local Notation continue_loop st := (ret (inl st)).
 Local Notation exit_loop st := (ret (inr st)).
-Local Notation rec_call := (trigger_inl1). 
+Local Notation rec_call := (trigger_inl1).
 
-Fixpoint meval_instr {E} `{ErrState -< E} (i : instr_r) (st: estate) :
-  itree (FCState +' E) estate := 
-  let R := st_cmd_map_r meval_instr in
+
+Local Notation gd := (p_globs pr).
+
+Definition sem_cond {E} `{ErrEvent -< E} (e:pexpr) (s: estate) :
+   itree E bool :=
+  iresult (fun s => sem_pexpr true gd s e >>r= to_bool) s.
+
+Definition sem_bound {E} `{ErrEvent -< E} (e:pexpr) (s: estate) :
+   itree E Z :=
+  iresult (fun s => sem_pexpr true gd s e >>r= to_int) s.
+
+Fixpoint meval_instr {E} `{ErrEvent -< E} (i : instr_r) (s1: estate) :
+  itree (FCState +' E) estate :=
+(*  let R := st_cmd_map_r meval_instr in *)
+  let R := (fun c s => rec_call (FLCode c s)) in
   match i with
-  | Cassgn x tg ty e => err_mk_AssgnE x tg ty e st
+  | Cassgn x tg ty e => iresult (eval_assgn x tg ty e) s1
+  | Copn xs tg o es => iresult (fun s1 => sem_sopn gd o s1 xs es) s1
+  | Csyscall xs o es => iresult (eval_syscall xs o es) s1
+  | Cif e c1 c2 =>
+      b <- sem_cond e s1;;
+      if b then R c1 s1 else R c2 s1
+  | Cwhile a c1 e c2 =>
+      ITree.iter (fun s1 =>
+           s2 <- R c1 s1 ;;
+           b <- sem_cond e s2 ;;
+           if b then s3 <- R c2 s2 ;; continue_loop s3
+           else exit_loop s2) s1
+  | Cfor i (d, lo, hi) c =>
+     vlo <- sem_bound lo s1 ;;
+     vhi <- sem_bound hi s1 ;;
+     eval_for R i c (wrange d vlo vhi) s1
+
+  | Ccall xs fn args =>
+      vargs <- isem_pexprs  (~~direct_call) gd s1 args;;
+      res <- rec_call (FFCall (escs s1) (emem s1) fn vargs);;
+      let: (scs2, m2, vs) := res in
+      iwrite_lvals (~~direct_call) gd (with_scs (with_mem s1 m2) scs2) xs vs
+end.
+
+
+err_mk_AssgnE x tg ty e st
   | Copn xs tg o es => err_mk_OpnE xs tg o es st
-  | Csyscall xs o es => err_mk_SyscallE xs o es st                          
-                                        
+  | Csyscall xs o es => err_mk_SyscallE xs o es st
+
   | Cif e c1 c2 =>
       b <- err_mk_EvalCond e st ;;
-      if b then R c1 st else R c2 st 
-                            
-  | Cfor i (d, lo, hi) c => 
+      if b then R c1 st else R c2 st
+
+  | Cfor i (d, lo, hi) c =>
           vlo <- err_mk_EvalBound lo st ;;
           vhi <- err_mk_EvalBound hi st ;;
           eval_for R i c (wrange d vlo vhi) st
 
-  | Cwhile a c1 e c2 => 
+  | Cwhile a c1 e c2 =>
       ITree.iter (fun st0 =>
-           st1 <- R c1 st0 ;;          
+           st1 <- R c1 st0 ;;
            b <- err_mk_EvalCond e st1 ;;
            if b then st2 <- R c2 st1 ;; continue_loop st2
            else exit_loop st1) st
-  
-  | Ccall xs fn es => rec_call (FFCall xs fn es st)      
+
+  | Ccall xs fn es => rec_call (FFCall xs fn es st)
   end.
 
-Definition meval_fcall {E} `{ErrState -< E}
+Definition meval_fcall {E} `{ErrEvent -< E}
   (xs: lvals) (fn: funname) (es: pexprs) (st0: estate) :
   itree (FCState +' E) estate :=
   va <- err_eval_Args fn es st0 ;;
@@ -488,22 +561,22 @@ Definition meval_fcall {E} `{ErrState -< E}
   vs <- err_return_val fn st2 ;;
   err_reinstate_caller fn xs vs st2 st0.
 
-Definition meval_cstate {E} `{ErrState -< E} :
-  FCState ~> itree (FCState +' E) :=           
+Definition meval_cstate {E} `{ErrEvent -< E} :
+  FCState ~> itree (FCState +' E) :=
   fun _ fs => match fs with
               | FLCode c st => st_cmd_map_r meval_instr c st
-              | FFCall xs fn es st => meval_fcall xs fn es st      
-              end.      
+              | FFCall xs fn es st => meval_fcall xs fn es st
+              end.
 
-Definition mevalE_cmd {E} `{ErrState -< E} (c: cmd) (st: estate) :
+Definition mevalE_cmd {E} `{ErrEvent -< E} (c: cmd) (st: estate) :
   itree E estate :=
   mrec meval_cstate (FLCode c st).
 
-Definition meval_cmd {E} (c: cmd) (st: estate) : itree E (option estate) := 
+Definition meval_cmd {E} (c: cmd) (st: estate) : itree E (option estate) :=
   @interp_Err E estate (mevalE_cmd c st).
 
-Definition mevalE_fun {E} `{ErrState -< E} :
-  (funname * (values * estate)) -> 
+Definition mevalE_fun {E} `{ErrEvent -< E} :
+  (funname * (values * estate)) ->
   itree E (values * estate) :=
   fun fvst =>
     let '(fn, (va, st)) := fvst in
@@ -513,7 +586,7 @@ Definition mevalE_fun {E} `{ErrState -< E} :
     vs <- err_return_val fn st2 ;;
     ret (vs, st2).
 
-Definition meval_fun_ {E} `{ErrState -< E}
+Definition meval_fun_ {E} `{ErrEvent -< E}
   (fn: funname) (va: values) (st0: estate) :
   itree (FCState +' E) (values * estate) :=
   st1 <- err_init_state fn va st0 ;;
